CoqOfRust/alloc/simulations/vec.v
@@ -1,0 +1,53 @@
+Require Import CoqOfRust.CoqOfRust.
+Require Import simulations.M.
+Import simulations.M.Notations.
+Require Import CoqOfRust.core.simulations.eq.
+
+Module List.
+  Fixpoint last_error {A : Set} (l : list A) : option A :=
+    match l with
+    | [] => None
+    | x :: [] => Some x
+    | x :: xs => last_error xs
+    end.
+End List.
+
+Definition first_mut {A : Set} : LensOption.t (list A) A :=
+  {|
+    LensOption.read l := List.hd_error l;
+    LensOption.write l x :=
+      match l with
+      | [] => None
+      | _ :: xs => Some (x :: xs)
+      end
+  |}.
+
+Definition last_mut {A : Set} : LensOption.t (list A) A :=
+  {|
+    LensOption.read l := List.last_error l;
+    LensOption.write l x :=
+      match List.last_error l with
+      | None => None
+      | Some _ => Some (List.app (List.removelast l) [x])
+      end
+  |}.
+
+Definition pop_front {A : Set} (self : list A) : option A * list A :=
+  match self with
+  | [] => (None, self)
+  | x :: xs => (Some x, xs)
+  end.
+
+Definition pop {A : Set} (self : list A) : option A * list A :=
+  match List.last_error self with
+  | None => (None, self)
+  | Some x =>
+    (Some x, List.removelast self)
+  end.
+
+Module ImplEq.
+  Global Instance I (A : Set) `{Eq.Trait A} :
+    Eq.Trait (list A) := {
+      eqb := List.eqb (Eq.eqb);
+    }.
+End ImplEq.
