CoqOfRust/core/simulations/bool.v
@@ -4,43 +4,43 @@ Import simulations.M.Notations.
 Require Import CoqOfRust.core.simulations.eq.
 
 Module Bool.
-  Definition and {State} (x y : MS? State bool) : MS? State bool :=
-    letS? a := x in
+  Definition and {State} (x y : MS! State bool) : MS! State bool :=
+    letS! a := x in
     if negb a
     then
-      returnS? false
+      returnS! false
     else
-      letS? b := y in
-      returnS? b.
+      letS! b := y in
+      returnS! b.
 
-  Definition or {State} (x y : MS? State bool) : MS? State bool :=
-    letS? a := x in
+  Definition or {State} (x y : MS! State bool) : MS! State bool :=
+    letS! a := x in
     if a
-    then returnS? true
+    then returnS! true
     else
-      letS? b := y in
-      returnS? (a && b)%bool.
+      letS! b := y in
+      returnS! (a && b)%bool.
 
-  Definition not {State} (x : MS? State bool) : MS? State bool :=
-    letS? a := x in
-    returnS? (negb a).
+  Definition not {State} (x : MS! State bool) : MS! State bool :=
+    letS! a := x in
+    returnS! (negb a).
 
   Definition if_then_else
         {State A}
-        (b : MS? State bool)
-        (x y : MS? State A) :
-        MS? State A :=
-    letS? b := b in
+        (b : MS! State bool)
+        (x y : MS! State A) :
+        MS! State A :=
+    letS! b := b in
     if b
     then x
     else y.
 End Bool.
 
 Module Notations.
-  Infix "&&S?" := Bool.and (at level 40, left associativity) : bool_scope.
-  Infix "||S?" := Bool.or (at level 50, left associativity) : bool_scope.
-  Notation "'notS?' b" := (Bool.not b) (at level 60).
-  Notation "'ifS?' b 'then' x 'else' y" := (Bool.if_then_else b x y) (at level 200, right associativity).
+  Infix "&&S!" := Bool.and (at level 40, left associativity) : bool_scope.
+  Infix "||S!" := Bool.or (at level 50, left associativity) : bool_scope.
+  Notation "'notS!' b" := (Bool.not b) (at level 60).
+  Notation "'ifS!' b 'then' x 'else' y" := (Bool.if_then_else b x y) (at level 200, right associativity).
 End Notations.
 
 Module ImplEq.
