CoqOfRust/core/simulations/slice.v
@@ -1,0 +1,20 @@
+Require Import CoqOfRust.CoqOfRust.
+Require Import simulations.M.
+Import simulations.M.Notations.
+Require Import CoqOfRust.core.simulations.eq.
+
+Definition contains {A : Set} `{Eq.Trait A} (self : list A) (x : A) : bool :=
+  List.existsb (Eq.eqb x) self.
+
+Definition swap {A : Set} (self : list A) (a b : Z) : M! (list A) :=
+  let a := Z.to_nat a in
+  let b := Z.to_nat b in
+  let x := List.nth_error self a in
+  let y := List.nth_error self b in
+  match x, y with
+  | Some x, Some y =>
+    let self := List.replace_at self a y in
+    let self := List.replace_at self b x in
+    return! self
+  | _, _ => panic! "swap: index out of bounds"
+  end.
